Fixed 4a verified by Dafny

LAB3/Fact.dfy
@@ -1,13 +1,20 @@
 method ComputeFact(n : nat) returns (res : nat)
-  requires n > 0;
-  ensures res == fact(n);
- {
-  res := 1;
-  var i := 2;
-  while (i <= n) 
-  {
-    res := res * i;
-    i := i + 1;
-  }
- }
- 
+requires n > 0;
+ensures res == fact(n);
+{
+	res := 1;
+	var i := 2;
+	while (i <= n)
+	invariant (i <= n + 1) && res == fact(i-1);
+	decreases (n - i);
+	{
+		res := res * i;
+		i := i + 1;
+	}
+}
+
+function fact(m : nat) : nat
+requires m > 0;
+{
+	if (m == 1) then 1 else m * fact(m - 1)
+}
